Pull dependencies back

treiber.v
@@ -1,9 +1,204 @@
 From iris.program_logic Require Export weakestpre.
 From iris.heap_lang Require Export lang.
 From iris.heap_lang Require Import proofmode notation.
-From iris.algebra Require Import upred gmap dec_agree upred_big_op.
-From iris.program_logic Require Import auth.
-From iris.tests Require Import treiber_stack atomic misc.
+From iris.algebra Require Import auth upred gmap dec_agree upred_big_op.
+From iris_atomic Require Import atomic misc.
+
+Definition new_stack: val := λ: <>, ref (ref NONE).
+
+Definition push: val :=
+  rec: "push" "s" "x" :=
+      let: "hd" := !"s" in
+      let: "s'" := ref SOME ("x", "hd") in
+      if: CAS "s" "hd" "s'"
+        then #()
+        else "push" "s" "x".
+
+Definition pop: val :=
+  rec: "pop" "s" :=
+      let: "hd" := !"s" in
+      match: !"hd" with
+        SOME "cell" =>
+        if: CAS "s" "hd" (Snd "cell")
+          then SOME (Fst "cell")
+          else "pop" "s"
+      | NONE => NONE
+      end.
+
+Definition iter: val :=
+  rec: "iter" "hd" "f" :=
+      match: !"hd" with
+        NONE => #()
+      | SOME "cell" => "f" (Fst "cell") ;; "iter" (Snd "cell") "f"
+      end.
+
+Global Opaque new_stack push pop iter.
+
+Section proof.
+  Context `{!heapG Σ} (N: namespace).
+
+  Fixpoint is_list (hd: loc) (xs: list val) : iProp Σ :=
+    match xs with
+    | [] => (∃ q, hd ↦{ q } NONEV)%I
+    | x :: xs => (∃ (hd': loc) q, hd ↦{ q } SOMEV (x, #hd') ★ is_list hd' xs)%I
+    end.
+
+  Lemma dup_is_list : ∀ xs hd,
+    heap_ctx ★ is_list hd xs ⊢ is_list hd xs ★ is_list hd xs.
+  Proof.
+    induction xs as [|y xs' IHxs'].
+    - iIntros (hd) "(#? & Hs)".
+      simpl. iDestruct "Hs" as (q) "[Hhd Hhd']". iSplitL "Hhd"; eauto.
+    - iIntros (hd) "(#? & Hs)". simpl.
+      iDestruct "Hs" as (hd' q) "([Hhd Hhd'] & Hs')".
+      iDestruct (IHxs' with "[Hs']") as "[Hs1 Hs2]"; first by iFrame.
+      iSplitL "Hhd Hs1"; iExists hd', (q / 2)%Qp; by iFrame.
+  Qed.
+
+  Lemma uniq_is_list:
+    ∀ xs ys hd, heap_ctx ★ is_list hd xs ★ is_list hd ys ⊢ xs = ys.
+  Proof.
+    induction xs as [|x xs' IHxs'].
+    - induction ys as [|y ys' IHys'].
+      + auto.
+      + iIntros (hd) "(#? & Hxs & Hys)".
+        simpl. iDestruct "Hys" as (hd' ?) "(Hhd & Hys')".
+        iExFalso. iDestruct "Hxs" as (?) "Hhd'".
+        iDestruct (heap_mapsto_op_1 with "[Hhd Hhd']") as "[% _]".
+        { iSplitL "Hhd"; done. }
+        done.
+    - induction ys as [|y ys' IHys'].
+      + iIntros (hd) "(#? & Hxs & Hys)".
+        simpl.
+        iExFalso. iDestruct "Hxs" as (? ?) "(Hhd & _)".
+        iDestruct "Hys" as (?) "Hhd'".
+        iDestruct (heap_mapsto_op_1 with "[Hhd Hhd']") as "[% _]".
+        { iSplitL "Hhd"; done. }
+        done.
+      + iIntros (hd) "(#? & Hxs & Hys)".
+        simpl. iDestruct "Hxs" as (? ?) "(Hhd & Hxs')".
+        iDestruct "Hys" as (? ?) "(Hhd' & Hys')".
+        iDestruct (heap_mapsto_op_1 with "[Hhd Hhd']") as "[% _]".
+        { iSplitL "Hhd"; done. }
+        inversion H3. (* FIXME: name *)
+        subst. iDestruct (IHxs' with "[Hxs' Hys']") as "%"; first by iFrame.
+        by subst.
+  Qed.
+
+  Definition is_stack (s: loc) xs: iProp Σ := (∃ hd: loc, s ↦ #hd ★ is_list hd xs)%I.
+
+  Global Instance is_list_timeless xs hd: TimelessP (is_list hd xs).
+  Proof. generalize hd. induction xs; apply _. Qed.
+
+  Global Instance is_stack_timeless xs hd: TimelessP (is_stack hd xs).
+  Proof. generalize hd. induction xs; apply _. Qed.
+
+  Lemma new_stack_spec:
+    ∀ (Φ: val → iProp Σ),
+      heapN ⊥ N →
+      heap_ctx ★ (∀ s, is_stack s [] -★ Φ #s) ⊢ WP new_stack #() {{ Φ }}.
+  Proof.
+    iIntros (Φ HN) "[#Hh HΦ]". wp_seq.
+    wp_bind (ref NONE)%E. wp_alloc l as "Hl".
+    wp_alloc l' as "Hl'".
+    iApply "HΦ". rewrite /is_stack. iExists l.
+    iFrame. by iExists 1%Qp.
+  Qed.
+
+  Definition push_triple (s: loc) (x: val) :=
+    atomic_triple (fun xs_hd: list val * loc =>
+                     let '(xs, hd) := xs_hd in s ↦ #hd ★ is_list hd xs)%I
+                  (fun xs_hd ret =>
+                     let '(xs, hd) := xs_hd in 
+                     ∃ hd': loc,
+                       ret = #() ★ s ↦ #hd' ★ hd' ↦ SOMEV (x, #hd) ★ is_list hd xs)%I
+                  (nclose heapN)
+                  ⊤
+                  (push #s x).
+  
+  Lemma push_atomic_spec (s: loc) (x: val) :
+    heapN ⊥ N → heap_ctx ⊢ push_triple s x.
+  Proof.
+    iIntros (HN) "#?". rewrite /push_triple /atomic_triple.
+    iIntros (P Q) "#Hvs".
+    iLöb as "IH". iIntros "!# HP". wp_rec.
+    wp_let. wp_bind (! _)%E.
+    iVs ("Hvs" with "HP") as ([xs hd]) "[[Hs Hhd] [Hvs' _]]".
+    wp_load. iVs ("Hvs'" with "[Hs Hhd]") as "HP"; first by iFrame.
+    iVsIntro. wp_let. wp_alloc l as "Hl". wp_let.
+    wp_bind (CAS _ _ _)%E.
+    iVs ("Hvs" with "HP") as ([xs' hd']) "[[Hs Hhd'] Hvs']".
+    destruct (decide (hd = hd')) as [->|Hneq].
+    * wp_cas_suc. iDestruct "Hvs'" as "[_ Hvs']".
+      iVs ("Hvs'" $! #() with "[-]") as "HQ".
+      { iExists l. iSplitR; first done. by iFrame. }
+      iVsIntro. wp_if. iVsIntro. eauto.
+    * wp_cas_fail.
+      iDestruct "Hvs'" as "[Hvs' _]".
+      iVs ("Hvs'" with "[-]") as "HP"; first by iFrame.
+      iVsIntro. wp_if. by iApply "IH".
+  Qed.
+
+  Definition pop_triple (s: loc) :=
+    atomic_triple (fun xs_hd: list val * loc =>
+                     let '(xs, hd) := xs_hd in s ↦ #hd ★ is_list hd xs)%I
+                  (fun xs_hd ret =>
+                     let '(xs, hd) := xs_hd in
+                     (ret = NONEV ★ xs = [] ★ s ↦ #hd ★ is_list hd []) ∨
+                     (∃ x q (hd': loc) xs', hd ↦{q} SOMEV (x, #hd') ★ ret = SOMEV x ★
+                                            xs = x :: xs' ★ s ↦ #hd' ★ is_list hd' xs'))%I
+                  (nclose heapN)
+                  ⊤
+                  (pop #s).
+
+  Lemma pop_atomic_spec (s: loc):
+    heapN ⊥ N → heap_ctx ⊢ pop_triple s.
+  Proof.
+    iIntros (HN) "#?".
+    rewrite /pop_triple /atomic_triple.
+    iIntros (P Q) "#Hvs".
+    iLöb as "IH". iIntros "!# HP". wp_rec.
+    wp_bind (! _)%E.
+    iVs ("Hvs" with "HP") as ([xs hd]) "[[Hs Hhd] Hvs']".
+    destruct xs as [|y' xs'].
+    - simpl. wp_load. iDestruct "Hvs'" as "[_ Hvs']".
+      iDestruct "Hhd" as (q) "[Hhd Hhd']".
+      iVs ("Hvs'" $! NONEV with "[-Hhd]") as "HQ".
+      { iLeft. iSplit=>//. iSplit=>//. iFrame. eauto. }
+      iVsIntro. wp_let. wp_load. wp_match.
+      iVsIntro. eauto.
+    - simpl. iDestruct "Hhd" as (hd' q) "([[Hhd1 Hhd2] Hhd'] & Hxs')".
+      iDestruct (dup_is_list with "[Hxs']") as "[Hxs1 Hxs2]"; first by iFrame.
+      wp_load. iDestruct "Hvs'" as "[Hvs' _]".
+      iVs ("Hvs'" with "[-Hhd1 Hhd2 Hxs1]") as "HP".
+      { iFrame. iExists hd', (q / 2)%Qp. by iFrame. }
+      iVsIntro. wp_let. wp_load. wp_match. wp_proj.
+      wp_bind (CAS _ _ _). iVs ("Hvs" with "HP") as ([xs hd'']) "[[Hs Hhd''] Hvs']".
+      destruct (decide (hd = hd'')) as [->|Hneq].
+      + wp_cas_suc. iDestruct "Hvs'" as "[_ Hvs']".
+        iVs ("Hvs'" $! (SOMEV y') with "[-]") as "HQ".
+        { iRight. iExists y', (q / 2 / 2)%Qp, hd', xs'.
+          destruct xs as [|x' xs''].
+          - simpl. iDestruct "Hhd''" as (?) "H".
+            iExFalso. iDestruct (heap_mapsto_op_1 with "[Hhd1 H]") as "[% _]".
+            { iSplitL "Hhd1"; done. }
+            done.
+          - simpl. iDestruct "Hhd''" as (hd''' ?) "(Hhd'' & Hxs'')".
+            iDestruct (heap_mapsto_op_1 with "[Hhd1 Hhd'']") as "[% _]".
+            { iSplitL "Hhd1"; done. }
+            inversion H0. (* FIXME: bad naming *) subst.
+            iDestruct (uniq_is_list with "[Hxs1 Hxs'']") as "%"; first by iFrame. subst.
+            repeat (iSplitR "Hxs1 Hs"; first done).
+            iFrame. }
+        iVsIntro. wp_if. wp_proj. eauto.
+      + wp_cas_fail. iDestruct "Hvs'" as "[Hvs' _]".
+        iVs ("Hvs'" with "[-]") as "HP"; first by iFrame.
+        iVsIntro. wp_if. by iApply "IH".
+  Qed.
+
+End proof.
+
+
 
 Section defs.
   Context `{heapG Σ, !evidenceG loc val Σ} (N: namespace).
@@ -174,8 +369,7 @@ Lemma new_stack_spec' Φ RI:
             { rewrite /ev. eauto. }
             iFrame.
             iDestruct (big_sepM_insert_later (perR R) m) as "H"=>//.
-            rewrite (insert_singleton_op m)=>//.
-            iExists ({[hd' := (1%Qp, DecAgree x)]} ⋅ m).
+            iExists (<[hd' := (1%Qp, DecAgree x)]> m).
             iFrame. iApply "H". iFrame. iExists x.
             iFrame. rewrite /allocated. iSplitR "Hhd'1"; auto.
           }
@@ -222,3 +416,4 @@ Lemma new_stack_spec' Φ RI:
   Qed.
 
 End proofs.
+
