atomic_sync.v
@@ -2,9 +2,8 @@ From iris.program_logic Require Export weakestpre hoare.
 From iris.heap_lang Require Export lang.
 From iris.heap_lang Require Import proofmode notation.
 From iris.heap_lang.lib Require Import spin_lock.
-From iris.tests Require Import atomic misc.
 From iris.algebra Require Import dec_agree frac.
-From iris.program_logic Require Import auth.
+From iris_atomic Require Import atomic misc.
 
 Definition syncR := prodR fracR (dec_agreeR val).
 Class syncG Σ := sync_tokG :> inG Σ syncR.
