misc.v
@@ -1,0 +1,248 @@
+From iris.program_logic Require Export weakestpre.
+From iris.heap_lang Require Export lang.
+From iris.heap_lang Require Import proofmode notation.
+From iris.algebra Require Import auth frac gmap dec_agree upred_big_op.
+From iris.prelude Require Import countable.
+Import uPred.
+
+Section lemmas.
+  Lemma op_some: ∀ {A: cmraT} (a b: A), Some a ⋅ Some b = Some (a ⋅ b).
+  Proof. done. Qed.
+
+  Lemma invalid_plus: ∀ (q: Qp), ¬ ✓ (1 + q)%Qp.
+  Proof.
+    intros q H.
+    apply (Qp_not_plus_q_ge_1 q).
+    done.
+  Qed.
+
+  Lemma pair_l_frac_update (g g': val):
+    ((1 / 2)%Qp, DecAgree g) ⋅ ((1 / 2)%Qp, DecAgree g) ~~> ((1 / 2)%Qp, DecAgree g') ⋅ ((1 / 2)%Qp, DecAgree g').
+  Proof.
+    repeat rewrite pair_op dec_agree_idemp.
+    rewrite frac_op' Qp_div_2.
+    eapply cmra_update_exclusive.
+    done.
+  Qed.
+  
+  Lemma pair_l_frac_op (p q: Qp) (g g': val):
+    (((p, DecAgree g') ⋅ (q, DecAgree g'))) ~~> ((p + q)%Qp, DecAgree g').
+  Proof. by rewrite pair_op dec_agree_idemp frac_op'. Qed.
+
+  Lemma pair_l_frac_op' (p q: Qp) (g g': val):
+     ((p + q)%Qp, DecAgree g') ~~> (((p, DecAgree g') ⋅ (q, DecAgree g'))).
+  Proof. by rewrite pair_op dec_agree_idemp frac_op'. Qed.
+
+  Lemma pair_l_frac_op_1' (g g': val):
+     (1%Qp, DecAgree g') ~~> (((1/2)%Qp, DecAgree g') ⋅ ((1/2)%Qp, DecAgree g')).
+  Proof. by rewrite pair_op dec_agree_idemp frac_op' Qp_div_2. Qed.
+  
+End lemmas.
+
+Section excl.
+  Context `{!inG Σ (exclR unitC)}.
+  Lemma excl_falso γ Q':
+    own γ (Excl ()) ★ own γ (Excl ()) ⊢ Q'.
+  Proof.
+    iIntros "[Ho1 Ho2]". iCombine "Ho1" "Ho2" as "Ho".
+    iExFalso. by iDestruct (own_valid with "Ho") as "%".
+  Qed.
+End excl.
+
+Section pair.
+  Context `{EqDecision A, !inG Σ (prodR fracR (dec_agreeR A))}.
+  
+  Lemma m_frag_agree γm (q1 q2: Qp) (a1 a2: A):
+    own γm (q1, DecAgree a1) ★ own γm (q2, DecAgree a2)
+    ⊢ |=r=> own γm ((q1 + q2)%Qp, DecAgree a1) ★ (a1 = a2).
+  Proof.
+    iIntros "[Ho Ho']".
+    destruct (decide (a1 = a2)) as [->|Hneq].
+    - iSplitL=>//.
+      iCombine "Ho" "Ho'" as "Ho".
+      iDestruct (own_update with "Ho") as "?"; last by iAssumption.
+      by rewrite pair_op frac_op' dec_agree_idemp.
+    - iCombine "Ho" "Ho'" as "Ho".
+      iDestruct (own_valid with "Ho") as %Hvalid.
+      exfalso. destruct Hvalid as [_ Hvalid].
+      simpl in Hvalid. apply dec_agree_op_inv in Hvalid. inversion Hvalid. subst. auto.
+  Qed.
+End pair.
+
+Section evidence.  
+  Context (K A: Type) `{Countable K, EqDecision A}.
+  Definition evkR := prodR fracR (dec_agreeR A).
+  Definition evmapR := gmapUR K evkR.
+  Definition evidenceR := authR evmapR.
+  Class evidenceG Σ := EvidenceG { evidence_G :> inG Σ evidenceR }.
+  Definition evidenceΣ : gFunctors := #[ GFunctor (constRF evidenceR) ].
+
+  Instance subG_evidenceΣ {Σ} : subG evidenceΣ Σ → evidenceG Σ.
+  Proof. intros [?%subG_inG _]%subG_inv. split; apply _. Qed.
+
+  Lemma map_agree_eq m m' (hd: K) (p q: Qp) (x y: A):
+    m !! hd = Some (p, DecAgree y) →
+    m = {[hd := (q, DecAgree x)]} ⋅ m' → x = y.
+  Proof.
+    intros H1 H2.
+    destruct (decide (x = y)) as [->|Hneq]=>//.
+    exfalso.
+    subst. rewrite lookup_op lookup_singleton in H1.
+    destruct (m' !! hd) as [[b [c|]]|] eqn:Heqn; rewrite Heqn in H1; inversion H1=>//.
+    destruct (decide (x = c)) as [->|Hneq3]=>//.
+    - rewrite dec_agree_idemp in H3. by inversion H3.
+    - rewrite dec_agree_ne in H3=>//.
+  Qed.
+
+  Lemma map_agree_somebot m m' (hd: K) (p q: Qp) (x: A):
+    m !! hd = Some (p, DecAgreeBot) → m' !! hd = None →
+    m = {[hd := (q, DecAgree x)]} ⋅ m' → False.
+  Proof.
+    intros H1 H2 H3. subst. rewrite lookup_op lookup_singleton in H1.
+    destruct (m' !! hd) as [[b [c|]]|] eqn:Heqn; rewrite Heqn in H1; inversion H1=>//.
+  Qed.
+
+  Lemma map_agree_none m m' (hd: K) (q: Qp) (x: A):
+    m !! hd = None → m = {[hd := (q, DecAgree x)]} ⋅ m' → False.
+  Proof.
+    intros H1 H2. subst. rewrite lookup_op lookup_singleton in H1.
+    destruct (m' !! hd)=>//.
+  Qed.
+
+  Context `{!inG Σ (authR evmapR)}.
+
+  Definition ev γm (k : K) (v: A) := (∃ q, own γm (◯ {[ k := (q, DecAgree v) ]}))%I.
+
+  Lemma evmap_alloc γm m k v:
+    m !! k = None →
+    own γm (● m) ⊢ |=r=> own γm (● (<[ k := (1%Qp, DecAgree v) ]> m) ⋅ ◯ {[ k := (1%Qp, DecAgree v) ]}).
+  Proof.
+    iIntros (?) "Hm".
+    iDestruct (own_update with "Hm") as "?"; last by iAssumption.
+    apply auth_update_alloc, alloc_local_update=>//.
+  Qed.
+  
+  Lemma map_agree_none' γm m hd x:
+    m !! hd = None →
+    own γm (● m) ★ ev γm hd x ⊢ False.
+  Proof.
+    iIntros (?) "[Hom Hev]". iDestruct "Hev" as (?) "Hfrag".
+    iCombine "Hom" "Hfrag" as "Hauth".
+    iDestruct (own_valid γm (● m ⋅ ◯ {[hd := (_, DecAgree x)]})
+               with "[Hauth]") as %Hvalid=>//.
+    iPureIntro.
+    apply auth_valid_discrete_2 in Hvalid as [[af Compose%leibniz_equiv_iff] Valid].
+    eapply (map_agree_none m)=>//.
+  Qed.
+  
+  Lemma map_agree_eq' γm m hd p x agy:
+    m !! hd = Some (p, agy) →
+    own γm (● m) ★ ev γm hd x ⊢ own γm (● m) ★ ev γm hd x ★ DecAgree x = agy.
+  Proof.
+    iIntros (?) "[Hom Hev]". iDestruct "Hev" as (?) "Hfrag".
+    iCombine "Hom" "Hfrag" as "Hauth".
+    iDestruct (own_valid γm (● m ⋅ ◯ {[hd := (_, DecAgree x)]})
+               with "[Hauth]") as %Hvalid=>//.
+    apply auth_valid_discrete_2 in Hvalid as [[af Compose%leibniz_equiv_iff] Valid].
+    destruct agy as [y|].
+    - iDestruct "Hauth" as "[? ?]". iFrame. iSplitL.
+      { rewrite /ev. eauto. }
+      iPureIntro. destruct (decide (x = y)); try by subst.
+      exfalso. apply n. eapply (map_agree_eq m)=>//. (* XXX: Why it is uPred M *)
+    - iAssert (✓ m)%I as "H"=>//. rewrite (gmap_validI m).
+      iDestruct ("H" $! hd) as "%".
+      exfalso. subst. rewrite H0 in H2.
+      by destruct H2 as [? ?].
+  Qed.
+
+  Lemma pack_ev γm k v q:
+    own γm (◯ {[ k := (q, DecAgree v) ]}) ⊢ ev γm k v.
+  Proof. iIntros "?". rewrite /ev. eauto. Qed.
+  
+  Lemma dup_ev γm hd y:
+    ev γm hd y ⊢ |=r=> ev γm hd y ★ ev γm hd y.
+  Proof.
+    rewrite /ev. iIntros "Hev". iDestruct "Hev" as (q) "Hev".
+    iAssert (|=r=> own γm (◯ {[hd := ((q/2)%Qp, DecAgree y)]} ⋅
+                           ◯ {[hd := ((q/2)%Qp, DecAgree y)]}))%I with "[Hev]" as "==>[Hev1 Hev2]".
+    { iDestruct (own_update with "Hev") as "?"; last by iAssumption.
+      rewrite <- auth_frag_op.
+      by rewrite op_singleton pair_op dec_agree_idemp  frac_op' Qp_div_2. }
+    iSplitL "Hev1"; eauto.
+  Qed.
+
+  Lemma evmap_frag_agree_split γm p q1 q2 (a1 a2: A):
+    own γm (◯ {[p := (q1, DecAgree a1)]}) ★
+    own γm (◯ {[p := (q2, DecAgree a2)]})
+    ⊢ |=r=> own γm (◯ {[p := (q1, DecAgree a1)]}) ★
+            own γm (◯ {[p := (q2, DecAgree a1)]}) ★ (a1 = a2).
+  Proof.
+    iIntros "[Ho Ho']".
+    destruct (decide (a1 = a2)) as [->|Hneq].
+    - by iFrame.
+    - iCombine "Ho" "Ho'" as "Ho".
+      iDestruct (own_valid with "Ho") as %Hvalid.
+      exfalso. rewrite <-(@auth_frag_op evmapR) in Hvalid.
+      rewrite op_singleton in Hvalid.
+      apply auth_valid_discrete in Hvalid. simpl in Hvalid.
+      apply singleton_valid in Hvalid.
+      destruct Hvalid as [_ Hvalid].
+      apply dec_agree_op_inv in Hvalid. inversion Hvalid. subst. auto.
+  Qed.
+
+  Lemma evmap_frag_agree γm p q1 q2 (a1 a2: A):
+    own γm (◯ {[p := (q1, DecAgree a1)]}) ★
+    own γm (◯ {[p := (q2, DecAgree a2)]})
+    ⊢ |=r=> own γm (◯ {[p := ((q1 + q2)%Qp, DecAgree a1)]}) ★ (a1 = a2).
+  Proof.
+    iIntros "Hos".
+    iDestruct (evmap_frag_agree_split with "Hos") as "==>[Ho1 [Ho2 %]]".
+    iCombine "Ho1" "Ho2" as "Ho". iSplitL; auto.
+    iDestruct (own_update with "Ho") as "?"; last by iAssumption.
+    rewrite <-(@auth_frag_op evmapR {[p := (q1, DecAgree a1)]} {[p := (q2, DecAgree a1)]}).
+    by rewrite op_singleton pair_op frac_op' dec_agree_idemp.
+  Qed.
+
+  Lemma ev_agree γm k v1 v2:
+    ev γm k v1 ★ ev γm k v2 ⊢ |=r=> ev γm k v1 ★ ev γm k v1 ★ v1 = v2.
+  Proof.
+    iIntros "[Hev1 Hev2]".
+    iDestruct "Hev1" as (?) "Hev1". iDestruct "Hev2" as (?) "Hev2".
+    iDestruct (evmap_frag_agree_split with "[-]") as "==>[Hev1 [Hev2 %]]"; first iFrame.
+    subst. iSplitL "Hev1"; rewrite /ev; eauto.
+  Qed.
+
+End evidence.
+
+Section heap_extra.
+  Context `{heapG Σ}.
+
+  Lemma bogus_heap p (q1 q2: Qp) a b:
+    ~((q1 + q2)%Qp ≤ 1%Qp)%Qc →
+    heap_ctx ★ p ↦{q1} a ★ p ↦{q2} b ⊢ False.
+  Proof.
+    iIntros (?) "(#Hh & Hp1 & Hp2)".
+    iCombine "Hp1" "Hp2" as "Hp".
+    iDestruct (heap_mapsto_op_1 with "Hp") as "[_ Hp]".
+    rewrite heap_mapsto_eq. iDestruct (own_valid with "Hp") as %H'.
+    apply singleton_valid in H'. by destruct H' as [H' _].
+  Qed.
+  
+End heap_extra.
+
+Section big_op_later.
+  Context {M : ucmraT}.
+  Context `{Countable K} {A : Type}.
+  Implicit Types m : gmap K A.
+  Implicit Types Φ Ψ : K → A → uPred M. 
+
+  Lemma big_sepM_delete_later Φ m i x :
+    m !! i = Some x →
+    ▷ ([★ map] k↦y ∈ m, Φ k y) ⊣⊢ ▷ Φ i x ★ ▷ [★ map] k↦y ∈ delete i m, Φ k y.
+  Proof. intros ?. rewrite big_sepM_delete=>//. apply later_sep. Qed.
+
+  Lemma big_sepM_insert_later Φ m i x :
+    m !! i = None →
+    ▷ ([★ map] k↦y ∈ <[i:=x]> m, Φ k y) ⊣⊢ ▷ Φ i x ★ ▷ [★ map] k↦y ∈ m, Φ k y.
+  Proof. intros ?. rewrite big_sepM_insert=>//. apply later_sep. Qed.
+End big_op_later.
