Makefile.coq
@@ -50,11 +50,11 @@ vo_to_obj = $(addsuffix .o,\
 ##########################
 
 COQLIBS?=\
-  -Q "." flatcomb
+  -Q "." iris_atomic
 COQCHKLIBS?=\
-  -R "." flatcomb
+  -R "." iris_atomic
 COQDOCLIBS?=\
-  -R "." flatcomb
+  -R "." iris_atomic
 
 ##########################
 #                        #
@@ -96,12 +96,13 @@ endif
 #                    #
 ######################
 
-VFILES:=simple_sync.v\
-  pair_cas.v\
+VFILES:=atomic.v\
+  simple_sync.v\
   flat.v\
   atomic_pair.v\
   atomic_sync.v\
-  treiber.v
+  treiber.v\
+  misc.v
 
 ifneq ($(filter-out archclean clean cleanall printenv,$(MAKECMDGOALS)),)
 -include $(addsuffix .d,$(VFILES))
@@ -191,22 +192,22 @@ userinstall:
 
 install:
 	cd "." && for i in $(VOFILES) $(VFILES) $(GLOBFILES) $(NATIVEFILES) $(CMOFILES) $(CMIFILES) $(CMAFILES); do \
-	 install -d "`dirname "$(DSTROOT)"$(COQLIBINSTALL)/flatcomb/$$i`"; \
-	 install -m 0644 $$i "$(DSTROOT)"$(COQLIBINSTALL)/flatcomb/$$i; \
+	 install -d "`dirname "$(DSTROOT)"$(COQLIBINSTALL)/iris_atomic/$$i`"; \
+	 install -m 0644 $$i "$(DSTROOT)"$(COQLIBINSTALL)/iris_atomic/$$i; \
 	done
 
 install-doc:
-	install -d "$(DSTROOT)"$(COQDOCINSTALL)/flatcomb/html
+	install -d "$(DSTROOT)"$(COQDOCINSTALL)/iris_atomic/html
 	for i in html/*; do \
-	 install -m 0644 $$i "$(DSTROOT)"$(COQDOCINSTALL)/flatcomb/$$i;\
+	 install -m 0644 $$i "$(DSTROOT)"$(COQDOCINSTALL)/iris_atomic/$$i;\
 	done
 
 uninstall_me.sh: Makefile
 	echo '#!/bin/sh' > $@
-	printf 'cd "$${DSTROOT}"$(COQLIBINSTALL)/flatcomb && rm -f $(VOFILES) $(VFILES) $(GLOBFILES) $(NATIVEFILES) $(CMOFILES) $(CMIFILES) $(CMAFILES) && find . -type d -and -empty -delete\ncd "$${DSTROOT}"$(COQLIBINSTALL) && find "flatcomb" -maxdepth 0 -and -empty -exec rmdir -p \{\} \;\n' >> "$@"
-	printf 'cd "$${DSTROOT}"$(COQDOCINSTALL)/flatcomb \\\n' >> "$@"
+	printf 'cd "$${DSTROOT}"$(COQLIBINSTALL)/iris_atomic && rm -f $(VOFILES) $(VFILES) $(GLOBFILES) $(NATIVEFILES) $(CMOFILES) $(CMIFILES) $(CMAFILES) && find . -type d -and -empty -delete\ncd "$${DSTROOT}"$(COQLIBINSTALL) && find "iris_atomic" -maxdepth 0 -and -empty -exec rmdir -p \{\} \;\n' >> "$@"
+	printf 'cd "$${DSTROOT}"$(COQDOCINSTALL)/iris_atomic \\\n' >> "$@"
 	printf '&& rm -f $(shell find "html" -maxdepth 1 -and -type f -print)\n' >> "$@"
-	printf 'cd "$${DSTROOT}"$(COQDOCINSTALL) && find flatcomb/html -maxdepth 0 -and -empty -exec rmdir -p \{\} \;\n' >> "$@"
+	printf 'cd "$${DSTROOT}"$(COQDOCINSTALL) && find iris_atomic/html -maxdepth 0 -and -empty -exec rmdir -p \{\} \;\n' >> "$@"
 	chmod +x $@
 
 uninstall: uninstall_me.sh
